typeの補題はおわったが、varが証明できない…

TaPL/code/chapter23.v
@@ -288,37 +288,14 @@ destruct HeqΓ.
     - destruct H1. right. exists (x [T']). constructor. auto.
 Qed.
 
-Fixpoint type_subst_in_list (n: nat) (S: type) (Γ: list env_elem) : list env_elem :=
+Fixpoint env_subst (n: nat) (S: type) (Γ: list env_elem) : list env_elem :=
 match Γ with
     | nil => nil
     | (env_var_bind X) :: Γ' 
-    => env_var_bind ([[[n |→ S]]] X) :: type_subst_in_list n S Γ'
-    | env_type_bind :: Γ' => env_type_bind :: (type_subst_in_list n S Γ')
+    => env_var_bind ([[[n |→ S]]] X) :: env_subst n S Γ'
+    | env_type_bind :: Γ' => env_type_bind :: (env_subst n S Γ')
 end.
 
-Lemma env_with_one_less_type_var: forall Γ' Γ Γ0 m S U, Γ = Γ' ++ env_type_bind :: Γ0
--> env Γ -> m = count_env_type_bind Γ'
--> U = type_shift 0 (m + 1) S -> env (env_reverse_shift m (type_subst_in_list m U Γ' ++ Γ0)).
-induction Γ'.
-- intros. simpl. simpl in H. rewrite H in H0. inversion H0.  admit.
-- intros. destruct a.
-    + simpl. rewrite H in H0. simpl in H0. inversion H0. constructor.
-    apply IHΓ' with (Γ:=Γ'++env_type_bind::Γ0)(S:=S). auto. auto. auto. auto.
-    + simpl. rewrite H in H0. simpl in H0. inversion H0. admit.
-Admitted.
-
-Lemma get_var_type_and_subst: forall Γ' k m Γ0 S T U, get_var_type k (Γ' ++ env_type_bind :: Γ0) = Some T 
--> env (Γ' ++ env_type_bind :: Γ0)
--> m = count_env_type_bind Γ' 
--> U = type_shift 0 (m + 1) S
--> get_var_type k (env_reverse_shift m (type_subst_in_list m U Γ' ++ Γ0)) = 
-Some (type_reverse_shift m ([[[m |→ U]]] T)).
-induction Γ'.
-- intros. simpl. admit.
-- intros. destruct a.
-    + simpl. admit.
-    + simpl. simpl in H. apply IHΓ' with (S:=S). auto. admit. admit. apply H2.
-Admitted.
 
 Lemma type_shift_double: forall T m n d, m >= n -> type_shift (m+1) d (type_shift n 1 T)
 = type_shift n 1 (type_shift m d T). induction T.
@@ -340,40 +317,43 @@ Lemma type_shift_double: forall T m n d, m >= n -> type_shift (m+1) d (type_shif
   apply H0 in H1. rewrite H1. reflexivity. 
 Qed.
 
-Lemma type_subst_dist_m: forall T c m U, type_shift (m+1) c ([[[m |→ U]]] T)
-= [[[m |→ type_shift (m+1) c U]]] (type_shift (m+1) c T). induction T.
+Lemma type_subst_dist_m: forall T m n U, m >= n -> type_shift (m+1) 1 ([[[n |→ U]]] T)
+= [[[n |→ type_shift (m+1) 1 U]]] (type_shift (m+1) 1 T). induction T.
 - intros. simpl. reflexivity.
-- intros. simpl. remember (n=?m) as b. destruct b. symmetry in Heqb.
-  apply Nat.eqb_eq in Heqb. subst. assert ((m+1<=?m)=false). apply Nat.leb_gt.
-  lia. rewrite H. simpl. assert ((m=?m)=true). apply Nat.eqb_eq. lia. rewrite H0.
-  reflexivity. remember (m+1<=?n) as b. destruct b. simpl. symmetry in Heqb0.
-  rewrite Heqb0. assert ((n+c =? m)=false). apply Nat.leb_le in Heqb0. apply Nat.eqb_neq.
-  lia. rewrite H. reflexivity. simpl. symmetry in Heqb0. rewrite Heqb0.
-  symmetry in Heqb. rewrite Heqb. reflexivity.
-- intros. simpl. rewrite IHT1. rewrite IHT2. reflexivity.
-- intros. simpl. pose proof (IHT c (m+1) (type_shift 0 1 U)).
-  pose proof (type_shift_double U (m+1) 0 c). assert (m+1>=0). lia. apply H0 in H1.
-  symmetry in H1. rewrite H1. assert (S m = m + 1). lia. rewrite H2. rewrite H. reflexivity.
+- intros. simpl. remember (n=?n0) as b. destruct b. symmetry in Heqb. apply Nat.eqb_eq in Heqb.
+  subst. assert ((m+1 <=?n0) = false). apply Nat.leb_gt. lia. rewrite H0. simpl. 
+  assert ((n0=?n0) = true). apply Nat.eqb_eq. reflexivity. rewrite H1. reflexivity.
+  remember (m+1 <=?n) as b. destruct b. symmetry in Heqb0. apply Nat.leb_le in Heqb0. simpl.
+  assert ((m+1 <=?n) = true). apply Nat.leb_le. auto. rewrite H0. assert ((n+1 =? n0) = false).
+  apply Nat.eqb_neq. lia. rewrite H1. reflexivity.
+  symmetry in Heqb0. apply Nat.leb_gt in Heqb0. symmetry in Heqb. apply Nat.eqb_neq in Heqb.
+  simpl. assert ((m+1 <=? n) = false). apply Nat.leb_gt. auto. assert ((n=?n0)=false). apply Nat.eqb_neq.
+  lia. rewrite H0. rewrite H1. reflexivity.
+- intros. simpl. rewrite IHT1. rewrite IHT2. reflexivity. auto. auto.
+- intros. simpl. pose proof (IHT (m+1) (n+1) (type_shift 0 1 U)).
+  pose proof (type_shift_double U (m+1) 0 1). assert (m+1>=0). lia. apply H1 in H2.
+  symmetry in H2. rewrite H2. assert (S n = n + 1). lia. rewrite H3. assert (m + 1 >= n + 1). lia.
+  apply H0 in H4. rewrite H4. reflexivity.
 Qed.
 
-Lemma type_subst_dist_zero: forall T c m U, 
-type_shift m c ([[[m |→ U]]] T)
-= [[[m + c |→ type_shift m c U]]] (type_shift m c T).
+Lemma type_subst_dist_zero: forall T n m U, m >= n ->
+type_shift n 1 ([[[m |→ U]]] T)
+= [[[m + 1 |→ type_shift n 1 U]]] (type_shift n 1 T).
 induction T.
 - intros. simpl. reflexivity.
-- intros. simpl. remember (n =? m) as b. destruct b. assert (n = m).
-  apply EqNat.beq_nat_eq in Heqb. apply Heqb. subst. assert (m <= m). lia. apply Compare_dec.leb_correct in H.
-  rewrite H. simpl. assert ((m+c =? m+c) = true). apply Nat.eqb_eq. reflexivity. rewrite H0.
-  reflexivity. simpl. remember (m <=? n) as b. destruct b. simpl. 
-  assert (n + c <> m + c). assert (n <> m). symmetry in Heqb. apply EqNat.beq_nat_false in Heqb.
-  auto. lia. apply Nat.eqb_neq in H. rewrite H. reflexivity. simpl.
-  assert (m > n). symmetry in Heqb0. apply Nat.leb_gt in Heqb0. lia. assert (n <> m + c).
-  lia. apply Nat.eqb_neq in H0. rewrite H0. reflexivity. 
-- intros. simpl. rewrite IHT1. rewrite IHT2. reflexivity.
-- intros. simpl. pose proof (IHT c (m+1) (type_shift 0 1 U)). 
-  pose proof (type_shift_double U m 0 c). assert (m >= 0). lia. apply H0 in H1. symmetry in H1.
-  rewrite H1. assert (S m = m + 1). lia. rewrite H2. rewrite H. assert (m + 1 + c = S (m + c)).
-  lia. rewrite H3. reflexivity.
+- intros. simpl. remember (n0 <=? n) as b. destruct b. symmetry in Heqb. simpl.
+  remember (n =? m) as b. destruct b. assert ((n+1 =?m+1) = true). apply Nat.eqb_eq.
+  symmetry in Heqb0. apply Nat.eqb_eq in Heqb0. lia. rewrite H0. reflexivity.
+  assert ((n+1=?m+1) = false). apply Nat.eqb_neq. symmetry in Heqb0. apply Nat.eqb_neq in Heqb0.
+  lia. rewrite H0. simpl. rewrite Heqb. reflexivity.
+  simpl. symmetry in Heqb. apply Nat.leb_gt in Heqb. assert ((n=?m)=false). apply Nat.eqb_neq. lia.
+  assert ((n=?m+1)=false). apply Nat.eqb_neq. lia. rewrite H0. rewrite H1. simpl.
+  apply Nat.leb_gt in Heqb. rewrite Heqb. reflexivity.
+- intros. simpl. rewrite IHT1. rewrite IHT2. reflexivity. auto. auto.
+- intros. simpl. pose proof (IHT (n+1) (m+1) (type_shift 0 1 U)). 
+  pose proof (type_shift_double U n 0 1). assert (n >= 0). lia. apply H1 in H2. symmetry in H2.
+  rewrite H2. assert (S m = m + 1). lia. rewrite H3. assert (S (m+1) = m + 1 + 1).
+  lia. rewrite H4. assert (m + 1 >= n + 1). lia. apply H0 in H5. rewrite H5. reflexivity.
 Qed.
 
 Lemma type_shift_inversion: forall T c, type_reverse_shift c (type_shift c 1 T) = T.
@@ -387,19 +367,52 @@ induction T.
 - intros. simpl. pose proof IHT (c+1). rewrite H. auto.
 Qed.
 
-Lemma type_shift_swap_m: forall T m n, m >= n -> 
-type_shift m 1 (type_reverse_shift n T) = type_reverse_shift n (type_shift (m+1) 1 T).
+Fixpoint has_free_var_in_type (m: nat) (T: type): bool :=
+  match T with
+  | Nat => false
+  | TVar k => if m =? k then true else false
+  | T1 → T2 => (has_free_var_in_type m T1) || (has_free_var_in_type m T2)
+  | ∀ T' => has_free_var_in_type (m + 1) T'
+end.
+
+Lemma free_var_in_type_shift_prep: forall T m n l, m >= l -> 
+(forall k, m > k -> k >= l -> has_free_var_in_type k T = false) ->
+(forall c, m + n > c -> c >= l -> has_free_var_in_type c (type_shift m n T) = false).
 induction T.
 - intros. simpl. reflexivity.
-- intros. simpl. remember (n0<=?n) as b. destruct b.
-    + simpl. symmetry in Heqb. apply Nat.leb_le in Heqb.
-    remember (m+1<=?n) as b. destruct b. symmetry in Heqb0. apply Nat.leb_le in Heqb0.
-    simpl. assert ((n0 <=? n+1)=true). apply Nat.leb_le. lia. rewrite H0.
-    assert ((m <=? Init.Nat.pred n) = true). apply Nat.leb_le. lia. rewrite H1.
-    assert (Init.Nat.pred n + 1 = Init.Nat.pred (n+1)). lia. rewrite H2. reflexivity.
-(* - intros. simpl. rewrite IHT1. rewrite IHT2. reflexivity. auto. auto.
-- intros. simpl. pose proof (IHT (m+1) (n+1)). rewrite H0. reflexivity. lia. *)
-Admitted. 
+- intros. simpl. remember (m <=? n) as b. destruct b. symmetry in Heqb. apply Nat.leb_le in Heqb.
+  simpl. assert ((c =? n + n0) = false). apply Nat.eqb_neq. lia. rewrite H3. reflexivity.
+  symmetry in Heqb. apply Nat.leb_gt in Heqb. assert (m > n). lia. simpl. remember (c =? n) as b. 
+  destruct b. symmetry in Heqb0. apply Nat.eqb_eq in Heqb0. subst. pose proof (H0 n H3 H2).
+  simpl in H4. assert ((n =? n)= true). apply Nat.eqb_eq. lia. rewrite H5 in H4. inversion H4.
+  reflexivity.
+- intros. simpl. rewrite IHT1 with (l:=l). rewrite IHT2 with (l:=l). simpl. reflexivity.
+  auto. intros. pose proof (H0 k H3 H4). simpl in H5. apply Bool.orb_false_elim in H5. destruct H5.
+  apply H6. auto. auto. auto. intros. pose proof (H0 k H3 H4). simpl in H5.
+  apply Bool.orb_false_elim in H5. destruct H5. auto. auto. auto.
+- intros. simpl. pose proof (IHT (m+1) n). simpl in H0. 
+assert (forall k, m + 1 > k -> k >= l + 1 -> has_free_var_in_type k T = false).
+intros. remember (k - 1) as k'. assert (k = k' + 1). lia. rewrite H6.
+pose proof (H0 k'). apply H7. lia. lia. assert (m + 1 >= l + 1). lia.
+pose proof (H3 (l+1) H5 H4 (c + 1)). apply H6. lia. lia.
+Qed.
+
+Lemma free_var_in_type_shift_prep_2: forall T l m n, m >= l ->
+has_free_var_in_type m T = false -> has_free_var_in_type (m + n) (type_shift l n T) = false.
+induction T.
+- intros. simpl. reflexivity.
+- intros. simpl. remember (l <=? n) as b. destruct b. simpl. assert ((m + n0 =? n + n0) = false).
+  simpl in H0. remember (m =? n) as b. destruct b. inversion H0. symmetry in Heqb0.
+  apply Nat.eqb_neq in Heqb0. apply Nat.eqb_neq. lia. rewrite H1. reflexivity.
+  symmetry in Heqb. apply Nat.leb_gt in Heqb. simpl. assert ((m + n0 =? n) = false).
+  apply Nat.eqb_neq. lia. rewrite H1. reflexivity.
+- intros. simpl. simpl in H0. rewrite IHT1. rewrite IHT2. simpl. reflexivity. auto.
+  apply Bool.orb_false_elim in H0. destruct H0. apply H1. auto. apply Bool.orb_false_elim in H0.
+  destruct H0. apply H0.
+- intros. simpl. simpl in H0. pose proof (IHT (l+1) (m+1) n). assert (m+1>=l+1).
+  lia. pose proof (H1 H2 H0). assert (m + 1 + n = m + n + 1). lia. rewrite H4 in H3.
+  apply H3.
+Qed.
 
 Lemma type_shift_zero: forall T c, type_shift c 0 T = T.
 induction T.
@@ -408,6 +421,122 @@ induction T.
   rewrite H. reflexivity. reflexivity.
 - intros. simpl. rewrite IHT1. rewrite IHT2. reflexivity.
 - intros. simpl. pose proof (IHT (c+1)). rewrite H. reflexivity.
+Qed.
+
+Lemma free_var_in_type_shift: forall c m T, 
+m > 0 -> has_free_var_in_type c (type_shift c m T) = false.
+intros. pose proof (free_var_in_type_shift_prep T c m c).
+apply H0. lia. intros. lia. lia. lia.
+Qed.
+
+Lemma free_var_in_type_shift_zero: forall m T, 
+has_free_var_in_type m (type_shift 0 (m+1) T) = false.
+intros. pose proof (free_var_in_type_shift_prep T 0 (m + 1) 0).
+apply H. lia. intros. lia. lia. lia. Qed.
+
+Lemma type_shift_inversion_reverse: forall T m, has_free_var_in_type m T = false ->
+type_shift m 1 (type_reverse_shift m T) = T.
+induction T.
+- intros. simpl. reflexivity.
+- intros. simpl in H. remember (m =? n) as b. destruct b. inversion H. symmetry in Heqb.
+  simpl. remember (m <=? n) as b. destruct b. symmetry in Heqb0. apply Nat.eqb_neq in Heqb.
+  apply Nat.leb_le in Heqb0. simpl. assert ((m <=? Init.Nat.pred n) = true).
+  apply Nat.leb_le. lia. rewrite H0. assert (Init.Nat.pred n + 1 = n). lia. rewrite H1. auto.
+  symmetry in Heqb0. apply Nat.leb_gt in Heqb0. simpl. assert ((m <=? n) = false).
+  apply Nat.leb_gt. auto. rewrite H0. reflexivity.
+- intros. simpl in H. apply Bool.orb_false_elim in H. destruct H. simpl.
+  rewrite IHT1. rewrite IHT2. reflexivity. auto. auto.
+- intros. simpl. simpl in H. pose proof (IHT (m + 1) H). rewrite H0. reflexivity.
+Qed.
+
+Lemma free_var_in_type_subst: forall T U m,
+has_free_var_in_type m U = false -> has_free_var_in_type m ([[[m |→ U]]] T) = false.
+induction T.
+- intros. simpl. reflexivity.
+- intros. simpl. remember (n =? m) as b. destruct b. symmetry in Heqb. apply Nat.eqb_eq in Heqb.
+  subst. auto. symmetry in Heqb. simpl. assert ((m =? n) = false).
+  apply Nat.eqb_neq in Heqb. apply Nat.eqb_neq. lia. rewrite H0. reflexivity.
+- intros. simpl. rewrite IHT1. rewrite IHT2. simpl. reflexivity. apply H. apply H.
+- intros. simpl. pose proof (IHT (type_shift 0 1 U) (m+1)). assert (S m = m + 1). lia.
+  rewrite H1. apply H0. pose proof (free_var_in_type_shift_prep_2 U 0 m 1). assert (m >= 0).
+  lia. apply H2. auto. auto.
+Qed.
+
+Lemma type_subst_no_free_var: forall T a U,
+has_free_var_in_type a T = false -> [[[a |→ U]]] T = T.
+induction T.
+- intros. simpl. auto.
+- intros. simpl. simpl in H. remember (a =? n) as b. destruct b. inversion H.
+  assert ((n =? a) = false). apply Nat.eqb_neq. symmetry in Heqb. apply Nat.eqb_neq in Heqb.
+  lia. rewrite H0. auto.
+- intros. simpl in H. apply Bool.orb_false_elim in H. destruct H. simpl.
+  rewrite IHT1. rewrite IHT2. auto. auto. auto.
+- intros. simpl. simpl in H. rewrite IHT. auto. assert (S a = a + 1). lia. rewrite H0. auto.
+Qed.
+
+Lemma type_subst_dist_subs: forall V a b T U, b > a
+-> has_free_var_in_type a T = false -> has_free_var_in_type a U = false
+-> [[[b |→ T]]] ([[[a |→ U]]] V) = [[[a |→ ([[[b |→ T]]] U)]]] ([[[b |→ T]]] V).
+induction V. 
+- intros. simpl. reflexivity.
+- intros. simpl. remember (n =? a) as c0. remember (n =? b) as c1. destruct c0, c1.
+  symmetry in Heqc0. symmetry in Heqc1. apply Nat.eqb_eq in Heqc0, Heqc1. lia.
+  simpl. symmetry in Heqc0. rewrite Heqc0. auto. simpl. symmetry in Heqc1.
+  rewrite Heqc1. rewrite type_subst_no_free_var. auto. auto.
+  simpl. symmetry in Heqc0. rewrite Heqc0. symmetry in Heqc1. rewrite Heqc1. auto. 
+- intros. simpl. rewrite IHV1. rewrite IHV2. auto. auto. auto. auto. auto. auto. auto.
+- intros. simpl. pose proof (IHV (S a) (S b) (type_shift 0 1 T) (type_shift 0 1 U)).
+  assert (type_shift 0 1 ([[[b |→ T]]] U) = [[[S b |→ type_shift 0 1 T]]] type_shift 0 1 U).
+  assert (S b = b + 1). lia. rewrite H3. apply type_subst_dist_zero. lia.
+  rewrite H3. rewrite H2. reflexivity. lia. assert (S a = a + 1). lia. rewrite H4.
+  apply free_var_in_type_shift_prep_2. lia. auto. assert (S a = a + 1). lia. rewrite H4.
+  apply free_var_in_type_shift_prep_2. lia. auto.
+Qed.
+
+Lemma type_shift_swap_m: forall T m n, m >= n -> has_free_var_in_type n T = false ->
+type_shift m 1 (type_reverse_shift n T) = type_reverse_shift n (type_shift (m+1) 1 T).
+induction T.
+- intros. simpl. reflexivity.
+- intros. simpl. remember (n0<=?n) as b. destruct b.
+    + simpl. symmetry in Heqb. apply Nat.leb_le in Heqb.
+    remember (m+1<=?n) as b. destruct b. symmetry in Heqb0. apply Nat.leb_le in Heqb0.
+    simpl. assert ((n0 <=? n+1)=true). apply Nat.leb_le. lia. rewrite H1.
+    assert ((m <=? Init.Nat.pred n) = true). apply Nat.leb_le. lia. rewrite H2.
+    assert (Init.Nat.pred n + 1 = Init.Nat.pred (n+1)). lia. rewrite H3. reflexivity.
+    simpl in H0. remember (n0 =? n) as b. destruct b. inversion H0. symmetry in Heqb1.
+    apply Nat.eqb_neq in Heqb1. simpl. assert ((n0 <=? n) = true). apply Nat.leb_le. lia.
+    rewrite H1. assert ((m <=? Init.Nat.pred n) = false). apply Nat.leb_gt.
+    symmetry in Heqb0. apply Nat.leb_gt in Heqb0. lia. rewrite H2. reflexivity.
+    + simpl. symmetry in Heqb. apply Nat.leb_gt in Heqb. assert ((m <=? n) = false).
+    apply Nat.leb_gt. lia. assert ((m+1<=?n)=false). apply Nat.leb_gt. lia. rewrite H1.
+    rewrite H2. simpl. assert ((n0 <=? n) = false). apply Nat.leb_gt. auto. rewrite H3.
+    reflexivity.
+- intros. simpl. rewrite IHT1. rewrite IHT2. reflexivity. auto. simpl in H0. 
+  apply Bool.orb_false_elim in H0. destruct H0. apply H1. auto.
+  simpl in H0. apply Bool.orb_false_elim in H0. destruct H0. apply H0.
+- intros. simpl. pose proof (IHT (m+1) (n+1)). rewrite H1. reflexivity. lia. simpl in H0. apply H0.
+Qed.
+
+Lemma type_shift_swap_zero: forall T m n, m >= n -> has_free_var_in_type m T = false ->
+type_shift n 1 (type_reverse_shift m T) = type_reverse_shift (m+1) (type_shift n 1 T).
+induction T.
+- intros. simpl. reflexivity.
+- intros. simpl in H0. remember (m =? n) as b. destruct b. inversion H0. symmetry in Heqb.
+  simpl. remember (n0 <=? n) as b. destruct b. symmetry in Heqb0. apply Nat.leb_le in Heqb0.
+  simpl. remember (m <=? n) as b. destruct b. symmetry in Heqb1. apply Nat.leb_le in Heqb1.
+  simpl. assert ((m + 1 <=? n + 1) = true). apply Nat.leb_le. lia. rewrite H1.
+  assert ((n0 <=? Init.Nat.pred n) = true). apply Nat.leb_le. apply Nat.eqb_neq in Heqb.
+  lia. rewrite H2. apply Nat.eqb_neq in Heqb. assert (Init.Nat.pred n + 1 = Init.Nat.pred (n + 1)).
+  lia. rewrite H3. reflexivity. simpl. symmetry in Heqb1. apply Nat.leb_gt in Heqb1.
+  assert ((m + 1 <=? n + 1) = false). apply Nat.leb_gt. lia. rewrite H1. assert ((n0 <=? n) = true).
+  apply Nat.leb_le. lia. rewrite H2. reflexivity. simpl. symmetry in Heqb0.
+  apply Nat.leb_gt in Heqb0. assert ((m <=? n) = false). apply Nat.leb_gt. lia.
+  assert ((m +1 <=? n) = false). apply Nat.leb_gt. lia. rewrite H1. rewrite H2. simpl.
+  assert ((n0 <=? n) = false). apply Nat.leb_gt. auto. rewrite H3. reflexivity.
+- intros. simpl in H0. apply Bool.orb_false_elim in H0. destruct H0. simpl. rewrite IHT1.
+  rewrite IHT2. reflexivity. apply H. apply H1. apply H. apply H0.
+- intros. simpl. pose proof (IHT (m+1) (n+1)). assert (m+1 >= n + 1). lia. apply H1 in H2.
+  rewrite H2. reflexivity. simpl in H0. apply H0.
 Qed.
 
 Lemma env_shift_zero: forall Γ, env_shift 0 0 Γ = Γ.
@@ -424,10 +553,135 @@ induction Γ.
   reflexivity. simpl. rewrite IHΓ. reflexivity.
 Qed.
 
+Lemma env_shift_inversion_reverse: forall Γ, env_shift 0 1 (env_reverse_shift 0 Γ) = Γ.
+induction Γ.
+- simpl. reflexivity.
+- destruct a. simpl. rewrite IHΓ. rewrite type_shift_inversion_reverse. auto. admit.
+  simpl. rewrite IHΓ. auto.
+Admitted.
+
+Lemma shift_combine: forall T c d e, shift c d (shift c e T) =
+shift c (d + e) T.
+induction T.
+- intros. simpl. auto.
+- intros. simpl. rewrite IHT. auto.
+- intros. simpl. rewrite IHT. auto.
+- intros. simpl. rewrite IHT1. rewrite IHT2. auto.
+- intros. simpl. remember (c <=? n) as b. destruct b. simpl. symmetry in Heqb.
+  apply Nat.leb_le in Heqb. assert ((c <=? n+e) = true). apply Nat.leb_le. lia.
+  rewrite H. assert (n + e + d = n + (d + e)). lia. rewrite H0. auto.
+  simpl. symmetry in Heqb. rewrite Heqb. auto.
+- intros. simpl. rewrite IHT. auto.
+- intros. simpl. rewrite IHT. auto.
+Qed.
+
+Lemma type_shift_combine: forall T c d e, type_shift c d (type_shift c e T) =
+type_shift c (d + e) T.
+induction T.
+- intros. simpl. auto.
+- intros. simpl. remember (c <=? n) as b. destruct b. simpl. assert ((c <=? n + e) = true).
+  apply Nat.leb_le. symmetry in Heqb. apply Nat.leb_le in Heqb. lia. rewrite H.
+  assert (n + e + d = (n + (d + e))). lia. rewrite H0. auto. simpl. symmetry in Heqb. rewrite Heqb.
+  auto.
+- intros. simpl. rewrite IHT1. rewrite IHT2. auto.
+- intros. simpl. rewrite IHT. auto.
+Qed.
+
+Lemma env_reverse_shift_split: forall m Γ Γ', env_reverse_shift m (Γ ++ Γ') =
+env_reverse_shift m Γ ++ env_reverse_shift m Γ'.
+intros ? ?. generalize dependent m. induction Γ.
+- intros. simpl. auto.
+- intros. destruct a. simpl. rewrite IHΓ. auto. simpl. rewrite IHΓ. auto.
+Qed.
+
+Lemma env_shift_split: forall c d Γ Γ', env_shift c d (Γ ++ Γ') =
+env_shift c d Γ ++ env_shift c d Γ'.
+intros ? ? ?.  generalize dependent c. generalize dependent d. induction Γ.
+- intros. simpl. auto.
+- intros. destruct a. simpl. rewrite IHΓ. auto. simpl. rewrite IHΓ. auto.
+Qed.
+
+Lemma env_shift_swap_zero: forall m Γ, env_shift 0 1 (env_reverse_shift m Γ) =
+env_reverse_shift (m+1) (env_shift 0 1 Γ).
+intros ? ?. generalize dependent m. induction Γ.
+- intros. simpl. auto.
+- intros. destruct a. simpl. rewrite IHΓ. rewrite type_shift_swap_zero. auto.
+  lia. admit. simpl. rewrite IHΓ. auto.
+Admitted.
+
+Lemma env_type_subst_zero: forall m U Γ, env_shift 0 1 (env_subst m U Γ)
+= env_subst (m+1) (type_shift 0 1 U) (env_shift 0 1 Γ).
+intros ? ? ?. generalize dependent m. generalize dependent U. induction Γ.
+- intros. simpl. auto.
+- intros. destruct a. simpl. rewrite type_subst_dist_zero. rewrite IHΓ. auto. lia. 
+  simpl. rewrite IHΓ. auto.
+Qed.
+
+Lemma count_env_type_bind_shift: forall c d Γ, count_env_type_bind Γ =
+count_env_type_bind (env_shift c d Γ). intros ? ? ?. generalize dependent d. 
+generalize dependent c. induction Γ. intros. simpl. auto. intros. destruct a. simpl. apply IHΓ.
+simpl. symmetry in IHΓ. rewrite IHΓ. auto. Qed.
+
+Lemma count_env_type_bind_reverse: forall m Γ, count_env_type_bind Γ =
+count_env_type_bind (env_reverse_shift m Γ). intros ? ?. generalize dependent m.
+induction Γ. intros. simpl. auto. intros. destruct a. simpl. apply IHΓ.
+simpl. symmetry in IHΓ. rewrite IHΓ. auto. Qed.
+
+Lemma count_env_var_bind_shift: forall c d Γ, count_env_var_bind Γ =
+count_env_var_bind (env_shift c d Γ). intros ? ? ?. generalize dependent d.
+generalize dependent c. induction Γ. intros. simpl. auto.
+intros. destruct a. simpl. rewrite IHΓ with (c:=c) (d:=d). auto. simpl. 
+rewrite IHΓ with (c:=c) (d:=d). auto. Qed. 
+
+Lemma env_shift_combine: forall c d e Γ, env_shift c d (env_shift c e Γ) =
+env_shift c (d + e) Γ. intros ? ? ? ?. generalize dependent e. generalize dependent d. 
+generalize dependent c. induction Γ.
+- intros. simpl. auto.
+- intros. destruct a. simpl. rewrite IHΓ. rewrite type_shift_combine. auto.
+  simpl. rewrite IHΓ. auto.
+Qed.
+
+Lemma env_with_one_less_type_var: forall Γ' Γ Γ0 m S U, 
+env Γ -> Γ = Γ' ++ env_type_bind :: Γ0 -> m = count_env_type_bind Γ'
+-> U = type_shift 0 (m + 1) S -> env (env_reverse_shift m (env_subst m U Γ' ++ Γ0)).
+intros ? ? ? ? ? ? ?. generalize dependent Γ'. generalize dependent Γ0.
+generalize dependent m. generalize dependent S. generalize dependent U. induction H.
+- intros. destruct Γ'. inversion H. simpl in H. inversion H.
+- intros. destruct Γ'. inversion H0. simpl. simpl in H1. rewrite H1.
+  rewrite env_shift_inversion. apply H. destruct e. simpl in H0. inversion H0. 
+  simpl in H0. simpl in H1. inversion H0. simpl. remember (count_env_type_bind Γ') as m'.
+  assert (env_reverse_shift 0 (env_shift 0 1 Γ) 
+  = env_reverse_shift 0 (Γ' ++ env_type_bind :: Γ0)). rewrite H4. auto.
+  rewrite env_shift_inversion in H3. rewrite env_reverse_shift_split in H3. simpl in H3.
+  pose proof (IHenv (type_shift 0 (m' + 1) S) S m' 
+  (env_reverse_shift 0 Γ0) (env_reverse_shift 0 Γ') H3).
+  assert (m' = count_env_type_bind (env_reverse_shift 0 Γ')). 
+  rewrite count_env_type_bind_reverse with (m:=0) in Heqm'. apply Heqm'.
+  assert (type_shift 0 (m' + 1) S = type_shift 0 (m' + 1) S). auto.
+  pose proof (H5 H6 H7). remember (env_reverse_shift m' (env_subst m' (type_shift 0 (m' + 1) S)
+  (env_reverse_shift 0 Γ') ++ env_reverse_shift 0 Γ0)) as Γ0'. assert (env (env_type_bind :: env_shift 0 1 Γ0')).
+  constructor. apply H8. rewrite HeqΓ0' in H9. rewrite env_shift_swap_zero in H9. rewrite env_shift_split in H9.
+  rewrite env_type_subst_zero in H9. symmetry in H1. rewrite H1 in H9. rewrite type_shift_combine in H9.
+  assert (1 + m = m + 1). lia. rewrite H10 in H9.
+  symmetry in H2. rewrite H2 in H9. rewrite env_shift_inversion_reverse in H9. rewrite env_shift_inversion_reverse in H9.
+  apply H9.
+- intros. destruct Γ'. inversion H0. destruct e. simpl in H0. inversion H0. simpl.
+  constructor. apply IHenv with (S:=S). auto. simpl in H1. auto. auto. simpl in H0. inversion H0.
+Qed.
+
+Lemma get_var_type_and_subst: forall T Γ' k m Γ0 S U, get_var_type k (Γ' ++ env_type_bind :: Γ0) = Some T 
+-> env (Γ' ++ env_type_bind :: Γ0)
+-> m = count_env_type_bind Γ' 
+-> U = type_shift 0 (m + 1) S
+-> get_var_type k (env_reverse_shift m (env_subst m U Γ' ++ Γ0)) = 
+Some (type_reverse_shift m ([[[m |→ U]]] T)).
+induction T.
+Admitted.
+
 Lemma th23_5_1_type_prep: forall Γ Γ' m t T S U, Γ' ++ env_type_bind :: Γ |- t : T ->
 m = count_env_type_bind Γ' ->
 U = type_shift 0 (m + 1) S ->
-env_reverse_shift m ((type_subst_in_list m U Γ') ++ Γ) |- (type_term_reverse_shift m ([[m |→ U]] t))
+env_reverse_shift m ((env_subst m U Γ') ++ Γ) |- (type_term_reverse_shift m ([[m |→ U]] t))
 : (type_reverse_shift m ([[[m |→ U]]] T)).
 intros ? ? ? ? ? ? ? ?. remember (Γ' ++ env_type_bind :: Γ) as Γ''.
 generalize dependent Γ'. generalize dependent Γ. generalize dependent m. generalize dependent S. generalize dependent U. 
@@ -450,27 +704,75 @@ simpl in H3. apply H3. rewrite HeqΓ''. auto. auto. auto.
   auto. auto. auto. auto.
   pose proof (IHtype_bind (type_shift 0 1 U) S (m + 1) (env_shift 0 1 Γ0) (env_type_bind :: (env_shift 0 1 Γ'))). assert (m + 1 + 1 = m + 2).
   lia. rewrite H4 in H3. assert (Datatypes.S m = m + 1). lia. rewrite H5. simpl in H3.
-  assert (env_reverse_shift (m + 1) (type_subst_in_list (m + 1) (type_shift 0 1 U) (env_shift 0 1 Γ') ++ env_shift 0 1 Γ0)
-  = env_shift 0 1 (env_reverse_shift m (type_subst_in_list m U Γ' ++ Γ0))).
-  admit. rewrite H6 in H3. apply H3. rewrite HeqΓ''. admit. admit. admit.
-- intros. simpl. simpl in IHtype_bind. pose proof (TTApp (env_reverse_shift m (type_subst_in_list m U Γ' ++ Γ0)) 
+  assert (env_reverse_shift (m + 1) (env_subst (m + 1) (type_shift 0 1 U) (env_shift 0 1 Γ') ++ env_shift 0 1 Γ0)
+  = env_shift 0 1 (env_reverse_shift m (env_subst m U Γ' ++ Γ0))).
+  rewrite env_shift_swap_zero. assert (env_shift 0 1 (env_subst m U Γ' ++ Γ0) = 
+  env_subst (m + 1) (type_shift 0 1 U) (env_shift 0 1 Γ') ++ env_shift 0 1 Γ0).
+  rewrite env_shift_split. rewrite env_type_subst_zero. auto. rewrite H6. auto.
+  rewrite H6 in H3. apply H3. rewrite HeqΓ''. rewrite env_shift_split. simpl. auto. 
+  pose proof (count_env_type_bind_shift). symmetry in H7. rewrite H7. lia. rewrite H2.
+  rewrite type_shift_combine. assert (1 + (m + 1) = m + 2). lia. rewrite H7. auto.
+- intros. simpl. simpl in IHtype_bind. pose proof (TTApp (env_reverse_shift m (env_subst m U Γ' ++ Γ0)) 
 (type_term_reverse_shift m
 ([[m |→ U]] t)) (type_reverse_shift (m + 1)
 ([[[(m + 1)
  |→ type_shift 0 1 U]]] T)) (type_reverse_shift m
-([[[m |→ U]]] T'))). assert (env (env_reverse_shift m (type_subst_in_list m U Γ' ++ Γ0))).
+([[[m |→ U]]] T'))). assert (env (env_reverse_shift m (env_subst m U Γ' ++ Γ0))).
  apply env_with_one_less_type_var with (Γ:=Γ)(S:=S). auto. auto. auto. auto.
- assert (env_reverse_shift m (type_subst_in_list m U Γ' ++ Γ0)
+ assert (env_reverse_shift m (env_subst m U Γ' ++ Γ0)
  |- type_term_reverse_shift m
       ([[m |→ U]] t) : ∀ type_reverse_shift (m + 1)
       ([[[(m + 1)
        |→ type_shift 0 1 U]]] T)). 
 pose proof (IHtype_bind U S m Γ0 Γ'). assert (Datatypes.S m = m + 1). lia. rewrite H6 in H5.
-apply H5. auto. auto. auto. pose proof (H3 H4 H5). admit. (* hard *)
-Admitted.
-
-(* T <- T'(0) <- U(m) 
-T <- U(m+1) <- (T' <- U(m))(0) *)
+apply H5. auto. auto. auto. pose proof (H3 H4 H5). 
+remember (type_reverse_shift 0
+([[[0
+ |→ type_shift 0 1
+      (type_reverse_shift m ([[[m |→ U]]] T'))]]] 
+ type_reverse_shift (m + 1)
+   ([[[m + 1 |→ type_shift 0 1 U]]] T))) as leftT.
+remember ( type_reverse_shift m
+([[[m
+ |→ U]]] type_reverse_shift 0
+           ([[[0 |→ type_shift 0 1 T']]] T))) as rightT.
+assert (leftT = rightT).
+pose proof (type_shift_inversion leftT m).
+remember (type_reverse_shift m (type_shift m 1 leftT)) as leftT'. rewrite HeqleftT in HeqleftT'.
+remember ( ([[[0 |→ type_shift 0 1 (type_reverse_shift m ([[[m |→ U]]] T'))]]] 
+    type_reverse_shift (m + 1) ([[[m + 1 |→ type_shift 0 1 U]]] T))) as leftT''.
+pose proof (type_shift_swap_m leftT'' m 0). assert (m >= 0). lia.
+assert (has_free_var_in_type 0 leftT'' = false). 
+subst. apply free_var_in_type_subst. apply free_var_in_type_shift. lia. pose proof (H8 H9 H10). rewrite H11 in HeqleftT'.
+rewrite HeqleftT'' in HeqleftT'. remember (type_shift 0 1 (type_reverse_shift m ([[[m |→ U]]] T'))) as U'.
+remember (type_reverse_shift (m + 1) ([[[m + 1 |→ type_shift 0 1 U]]] T)) as leftT'''.
+pose proof (type_subst_dist_m leftT''' m 0 U'). apply H12 in H9. rewrite H9 in HeqleftT'.
+rewrite HeqleftT''' in HeqleftT'. rewrite H7 in HeqleftT'. 
+assert (type_shift 0 1 (type_reverse_shift m ([[[m |→ U]]] T')) =
+type_reverse_shift (m + 1) (type_shift 0 1 ([[[m |→ U]]] T'))). apply type_shift_swap_zero. lia.
+apply free_var_in_type_subst. rewrite H2. apply free_var_in_type_shift_zero.
+rewrite H13 in HeqU'. remember (type_shift (m + 1) 1 U') as U''. rewrite HeqU' in HeqU''.
+assert (U'' = (type_shift 0 1 ([[[m |→ U]]] T'))). rewrite HeqU''. apply type_shift_inversion_reverse.
+apply free_var_in_type_shift_prep_2. lia. apply free_var_in_type_subst. rewrite H2. apply free_var_in_type_shift_zero.
+remember (type_shift (m + 1) 1 (type_reverse_shift (m + 1) ([[[m + 1 |→ type_shift 0 1 U]]] T))) as T''.
+assert (T'' = [[[m + 1 |→ type_shift 0 1 U]]] T). rewrite HeqT''. apply type_shift_inversion_reverse.
+apply free_var_in_type_subst. apply free_var_in_type_shift_prep_2. lia. rewrite H2.
+apply free_var_in_type_shift_zero.
+pose proof free_var_in_type_shift.
+remember ([[[m |→ U]]] type_reverse_shift 0 ([[[0 |→ type_shift 0 1 T']]] T)) as rightT'.
+pose proof (type_shift_inversion rightT' 0). symmetry in H17. remember (type_shift 0 1 rightT') as rightT''.
+rewrite HeqrightT' in HeqrightT''. 
+pose proof (type_subst_dist_zero (type_reverse_shift 0 ([[[0 |→ type_shift 0 1 T']]] T)) 0 m U).
+assert (m>=0). lia. apply H18 in H19. rewrite H19 in HeqrightT''.
+remember (type_shift 0 1 (type_reverse_shift 0 ([[[0 |→ type_shift 0 1 T']]] T))) as V.
+assert (V = [[[0 |→ type_shift 0 1 T']]] T). rewrite HeqV. apply type_shift_inversion_reverse.
+apply free_var_in_type_subst. apply free_var_in_type_shift_zero. rewrite H20 in HeqrightT''.
+rewrite type_subst_dist_subs in HeqrightT''. rewrite type_subst_dist_zero in H14.
+rewrite HeqleftT'. rewrite H14. rewrite H15. rewrite HeqrightT. rewrite H17.
+rewrite HeqrightT''. reflexivity. lia. lia. apply free_var_in_type_shift_zero.
+apply free_var_in_type_shift_zero.  
+rewrite H7 in H6. apply H6.
+Qed.
 
 Lemma env_one_less_var_bind: forall Γ Γ' T, env (Γ ++ env_var_bind T :: Γ') -> env (Γ ++ Γ').
 induction Γ.
@@ -480,37 +782,55 @@ induction Γ.
     + subst. inversion H. subst. constructor. apply IHΓ with (T:=T). apply H1.
 Admitted.
 
-Lemma th23_5_1_var_prep: forall S Γ Γ' t T n m s, 
+Lemma th23_5_1_var_prep: forall S S' Γ Γ' t T n m s s', 
 Γ |- s : S ->
 n = count_env_var_bind Γ' ->
 m = count_env_type_bind Γ' ->
-Γ' ++ env_var_bind S :: (env_shift 0 m Γ) |- t : T ->
-Γ' ++ (env_shift 0 m Γ) |- reverse_shift n ([n |→ shift 0 (n + 1) s] t) : T.
-intros. remember (Γ' ++ env_var_bind S :: env_shift 0 m Γ) as Γ''. generalize dependent Γ'.
-generalize dependent s. generalize dependent S. generalize dependent Γ. 
-generalize dependent n. generalize dependent m. induction H2.
-- intros. simpl. constructor. apply env_one_less_var_bind with (T:=S). symmetry in HeqΓ''.
+S' = type_shift 0 m S ->
+s' = type_term_shift 0 m s ->
+Γ' ++ env_var_bind S' :: (env_shift 0 m Γ) |- t : T ->
+Γ' ++ (env_shift 0 m Γ) |- reverse_shift n ([n |→ shift 0 (n + 1) s'] t) : T.
+intros. remember (Γ' ++ env_var_bind S' :: env_shift 0 m Γ) as Γ''. generalize dependent Γ'.
+generalize dependent s. generalize dependent S. generalize dependent S'. generalize dependent Γ. 
+generalize dependent n. generalize dependent m. generalize dependent s'. induction H4.
+Admitted.
+- admit.
+- admit.
+- admit.
+- admit.
+- admit.
+- intros. simpl. constructor. admit.
+- admit.
+
+Admitted.
+(* - intros. simpl. constructor. apply env_one_less_var_bind with (T:=S). symmetry in HeqΓ''.
 rewrite HeqΓ''. auto.
 - intros. simpl. constructor. apply env_one_less_var_bind with (T:=S). 
   symmetry in HeqΓ''. rewrite HeqΓ''. apply H. apply IHtype_bind with (S:=S)(m:=m). auto. auto. auto. auto.
-- intros. simpl. remember (k =? n) as b. destruct b. admit. simpl. remember (n <=? k) as c. destruct c. 
+- intros. simpl. remember (k =? n) as b. destruct b. admit. simpl. remember (n <=? k) as c. destruct c.
   admit. admit.
 - intros. simpl. constructor. apply env_one_less_var_bind with (T:=S). symmetry in HeqΓ''. rewrite HeqΓ''. auto.
  rewrite HeqΓ'' in IHtype_bind.
  pose proof (IHtype_bind m (n + 1) Γ0 S s H0 (env_var_bind T1 :: Γ')).
  assert (Datatypes.S n = n + 1). lia. rewrite H5. simpl in H4.
  assert (shift 0 1 (shift 0 (n + 1) s) = shift 0 (n + 1 + 1) s).
- admit. rewrite H6. apply H4. auto. auto. auto. 
+ rewrite shift_combine. assert (1 + (n + 1) = (n + 1 + 1)). lia. rewrite H6. auto.
+ rewrite H6. apply H4. auto. auto. auto. 
 - intros. simpl. apply TApp' with (T11:=T11). apply env_one_less_var_bind with (T:=S). symmetry in HeqΓ''. rewrite HeqΓ''. auto.
   apply IHtype_bind1 with (S:=S). auto. auto. auto. auto. apply IHtype_bind2 with (S:=S).
   auto. auto. auto. auto.
 - intros. simpl. constructor. apply env_one_less_var_bind with (T:=S). symmetry in HeqΓ''. rewrite HeqΓ''. auto.
   pose proof (IHtype_bind (m + 1) n Γ0 S s H0 (env_type_bind :: (env_shift 0 1 Γ'))).
   simpl in H4. assert (env_shift 0 1 Γ' ++ env_shift 0 (m + 1) Γ0 = env_shift 0 1 (Γ' ++ env_shift 0 m Γ0)).
-  admit. rewrite H5 in H4. apply H4. admit. admit. admit.
+  rewrite env_shift_split. rewrite env_shift_combine. assert (m + 1 = 1 + m). lia. rewrite H5. auto.
+  rewrite H5 in H4. apply H4. 
+  pose proof (count_env_type_bind_shift). symmetry in H6. pose proof (count_env_var_bind_shift). 
+  symmetry in H7. rewrite H7. auto.
+  pose proof (count_env_type_bind_shift). symmetry in H6. rewrite H6. lia. 
+  rewrite HeqΓ''. rewrite env_shift_split. simpl. admit.
 - intros. simpl. constructor. apply env_one_less_var_bind with (T:=S). symmetry in HeqΓ''. rewrite HeqΓ''. auto.
   apply IHtype_bind with (S:=S). auto. auto. auto. auto.
-Admitted.
+Admitted. *)
 
 Theorem th23_5_1: forall Γ t T t', Γ |- t : T -> t -→ t' -> Γ |- t' : T.
 intros. generalize dependent t'. induction H.
